MemoNat/DArray.lean
@@ -1,0 +1,85 @@
+-- This intentionally only uses std, not mathlib
+import Std.Data.Array.Lemmas
+import Std.Data.Fin.Basic
+import Std.Tactic.Congr
+
+set_option autoImplicit false
+
+
+inductive Any.{u} : Type u
+| mk {α : Sort u} : α → Any
+
+protected abbrev Any.Sort : Any → Sort _
+| @mk α _ => α
+
+protected abbrev Any.val : (a : Any) → a.Sort
+| mk x => x
+
+theorem eq_req_any_val.{u} (a : Any) (α : Sort u) (h : Any.Sort a = α) : h ▸ Any.val a = a.val :=
+  sorry
+
+
+--  (_ : Any.Sort (Array.get (Array.push { arr := a, types := types }.arr (Any.mk x)) i) = C i.val) ▸
+    -- Any.val (Array.push a (Any.mk x))
+
+structure DArray.{u} (C : Nat → Type u) : Type (u+1):=
+  arr : Array Any.{u+1}
+  types : ∀ (i : Fin arr.size), (arr.get i).Sort = C i
+
+namespace DArray
+
+protected def empty {C} (cap : Nat) : DArray C :=
+  ⟨ Array.mkEmpty cap, λ i => Fin.elim0 i⟩
+
+def size {C} (a : DArray C) := a.arr.size
+
+protected def push {C} (a : DArray C) (x : C a.size) : DArray C :=
+  ⟨ a.arr.push (Any.mk x),
+   by 
+    cases a with | _ a types =>
+    dsimp
+    intro ⟨i, hi⟩
+    dsimp
+    rewrite [Array.get_push]
+    split
+    case inl hi2 =>
+      apply types
+    case inr hi2 =>
+      rewrite [Array.size_push, <- Nat.succ_eq_add_one] at hi
+      have : i = Array.size a :=
+        Nat.le_antisymm (Nat.le_of_lt_succ hi) (Nat.le_of_not_lt hi2)
+      cases this
+      rfl
+  ⟩
+
+protected theorem size_push {C} (a : DArray C) (x : C a.size) : (a.push x).size = a.size + 1 :=
+  Array.size_push _ _
+
+protected def get.{u} {C : Nat → Type u} (a : DArray C) (i : Fin a.size) : C i :=
+  let x : Any := Array.get a.arr i
+  a.types i ▸ x.val
+
+protected theorem get_push {C} (a : DArray C) (x : C a.size) (i : Fin (a.push x).size) :
+    (a.push x).get i =
+      if h : i < a.size
+      then a.get ⟨i, h⟩
+      else
+        have : size a = i := Nat.le_antisymm
+          (Nat.le_of_not_lt h)
+          (Nat.le_of_lt_succ (by simpa [a.size_push x] using i.isLt))
+        (this ▸ x : C i) := by
+  split 
+  case inl hi2 =>
+    rcases a with ⟨a, types⟩ 
+    unfold DArray.push
+    unfold DArray.get
+    dsimp
+    apply eq_of_heq
+
+    
+
+  -- rw [ SArray.get_push a.1 (Any.mk x) i hi ]
+  sorry
+  
+
+end DArray
